localchan.v
@@ -9,7 +9,10 @@ Set Default Proof Using "Type".
 (* To start off, let's try defining a blocking receive. *)
 
 Notation TryRecv e := (TryRecv e) (only parsing).
-Notation "'tryrecv' e" := (TryRecv e%E) (at level 10) : expr_scope.
+Notation "'tryrecv' e" := (TryRecv (LitV $ LitChan e%E)) (at level 10) : expr_scope.
+
+Notation NewCh := (NewCh) (only parsing).
+Notation "'newch' e" := (NewCh (LitV $ LitChan e%E)) (at level 10) : expr_scope.
 
 Definition recv : val :=
   rec: "loop" "c" :=
@@ -19,17 +22,46 @@ Definition recv : val :=
     | SOME "m" => "m"
     end.
 
+Definition threadpool := gmap chan_id (option (gset val)).
+
 (* In the language definitions, we had asynchronous channels.
   Here, we use invariant constructions to define _local channel assertions_. *)
 
+From iris.base_logic.lib Require Import invariants.
+From iris.program_logic Require Import ectx_lifting total_ectx_lifting.
+
 Section invariants.
 
-  Context `{LANG: irisG chan_lang Σ}.
+  Context `{LANG: irisG chan_lang Σ} (N : namespace).
   Notation iProp := (iProp Σ).
 
   Definition true : iProp := ⌜ True ⌝.
 
-  Lemma recv_spec c :
+  (* Definition newch_inv v : iProp := *)
+  (*   ( NONE)%I. *)
+
+  (* Definition wp_newch c : *)
+  (*   {{{ true }}} newch c {{{ RET #(); newch_inv v }}}. *)
+
+  Definition recv_inv v (P : iProp) (Q : threadpool -> chan_lang.val -> iProp) : iProp :=
+    (P ∗ ⌜v = NONE⌝ ∨ ∃ M m, Q M m ∗ ⌜v = SOMEV m⌝)%I.
+
+  Definition is_recv P Q v :=
+    inv N (recv_inv v P Q).
+
+  (* Section 7.2 Proof of blocking receive (10) *)
+  Lemma wp_tryrecv P (Q : threadpool -> chan_lang.val -> iProp) c :
+    {{{ P }}} tryrecv c {{{ v , RET v; is_recv P Q v }}}.
+  Proof.
+    iIntros (Φ) "P Q".
+    iApply wp_lift_atomic_head_step; [done|].
+    iIntros (σ1 ns κ κs nt) "Hσ !>". iSplit.
+    (* - first by euto with head_step. iMod "Q (tryrecv c)". *)
+    (*   unfold head_reducible. iExists _, _, _, _. iSimpl. *)
+    (*   iMod "Q".  as  "_". *)
+  Admitted.
+
+  Lemma recv_spec c (tp : list chan_lang.expr):
     {{{ True }}} recv c {{{ RET #(); true }}}.
   Proof.
   Abort.
