network_ra.v
@@ -1,0 +1,107 @@
+From iris.algebra Require Import gmap_view frac.
+From iris.algebra Require Export dfrac.
+From iris.bi.lib Require Import fractional.
+From iris.proofmode Require Import tactics.
+From iris.base_logic.lib Require Export own.
+From iris.prelude Require Import options.
+
+Class gen_networkGpreS (L V : Type) (Σ : gFunctors) `{Countable L} := {
+  gen_networkGpreS_inG :> inG Σ (gmap_viewR L (leibnizO V));
+}.
+
+Class gen_networkGS (L V : Type) (Σ : gFunctors) `{Countable L} := GenNetworkGS {
+  gen_network_inG :> gen_networkGpreS L V Σ;
+  gen_network_name : gname;
+}.
+Global Arguments GenNetworkGS L V Σ {_ _ _} _ : assert.
+Global Arguments gen_network_name {L V Σ _ _} _ : assert.
+
+Definition gen_networkΣ (L V : Type) `{Countable L} : gFunctors := #[
+  GFunctor (gmap_viewR L (leibnizO V))
+].
+
+Global Instance subG_gen_networkGpreS {Σ L V} `{Countable L} :
+  subG (gen_networkΣ L V) Σ → gen_networkGpreS L V Σ.
+Proof. solve_inG. Qed.
+
+Section definitions.
+  Context `{Countable L, hG : !gen_networkGS L V Σ}.
+
+  Definition gen_network_interp (σ : gmap L V) : iProp Σ :=
+    own (gen_network_name hG) (gmap_view_auth 1 (σ : gmap L (leibnizO V))).
+
+  Definition mapsto_def (l : L) (dq : dfrac) (v: V) : iProp Σ :=
+    own (gen_network_name hG) (gmap_view_frag l dq (v : leibnizO V)).
+  Definition mapsto_aux : seal (@mapsto_def). Proof. by eexists. Qed.
+  Definition mapsto := mapsto_aux.(unseal).
+  Definition mapsto_eq : @mapsto = @mapsto_def := mapsto_aux.(seal_eq).
+End definitions.
+
+Notation "l ↦{ dq } v" := (mapsto l dq v)
+  (at level 20, format "l  ↦{ dq }  v") : bi_scope.
+Notation "l ↦ v" := (mapsto l (DfracOwn 1) v)
+  (at level 20, format "l  ↦  v") : bi_scope.
+
+Section gen_network.
+  Context {L V} `{Countable L, !gen_networkGS L V Σ}.
+  Implicit Types (P Q : iProp Σ).
+  Implicit Types (Φ : V → iProp Σ).
+  Implicit Types (σ : gmap L V) (l : L) (v : V).
+
+  (** General properties of mapsto *)
+  Global Instance mapsto_timeless l dq v : Timeless (l ↦{dq} v).
+  Proof. rewrite mapsto_eq. apply _. Qed.
+
+  Lemma mapsto_valid_2 l dq1 dq2 v1 v2 : l ↦{dq1} v1 -∗ l ↦{dq2} v2 -∗ ⌜✓ (dq1 ⋅ dq2) ∧ v1 = v2⌝.
+  Proof.
+    rewrite mapsto_eq. iIntros "H1 H2".
+    iDestruct (own_valid_2 with "H1 H2") as %[??]%gmap_view_frag_op_valid_L.
+    auto.
+  Qed.
+  (** Almost all the time, this is all you really need. *)
+  Lemma mapsto_agree l dq1 dq2 v1 v2 : l ↦{dq1} v1 -∗ l ↦{dq2} v2 -∗ ⌜v1 = v2⌝.
+  Proof.
+    iIntros "H1 H2".
+    iDestruct (mapsto_valid_2 with "H1 H2") as %[_ ?].
+    done.
+  Qed.
+
+  (** Update lemmas *)
+  Lemma gen_network_alloc σ l v :
+    σ !! l = None →
+    gen_network_interp σ ==∗ gen_network_interp (<[l:=v]>σ) ∗ l ↦ v.
+  Proof.
+    iIntros (Hσl). rewrite /gen_network_interp mapsto_eq /mapsto_def /=.
+    iIntros "Hσ".
+    iMod (own_update with "Hσ") as "[Hσ Hl]".
+    { eapply (gmap_view_alloc _ l (DfracOwn 1)); done. }
+    iModIntro. iFrame.
+  Qed.
+
+  Lemma gen_network_valid σ l dq v : gen_network_interp σ -∗ l ↦{dq} v -∗ ⌜σ !! l = Some v⌝.
+  Proof.
+    iIntros "Hσ Hl".
+    rewrite /gen_network_interp mapsto_eq.
+    by iDestruct (own_valid_2 with "Hσ Hl") as %[??]%gmap_view_both_valid_L.
+  Qed.
+
+  Lemma gen_network_update σ l v1 v2 :
+    gen_network_interp σ -∗ l ↦ v1 ==∗ gen_network_interp (<[l:=v2]>σ) ∗ l ↦ v2.
+  Proof.
+    iIntros "Hσ Hl".
+    rewrite /gen_network_interp mapsto_eq /mapsto_def.
+    iDestruct (own_valid_2 with "Hσ Hl") as %[_ Hl]%gmap_view_both_valid_L.
+    iMod (own_update_2 with "Hσ Hl") as "[Hσ Hl]".
+    { eapply gmap_view_update. }
+    iModIntro. iFrame.
+  Qed.
+End gen_network.
+
+Lemma gen_network_init `{Countable L, !gen_networkGpreS L V Σ} σ :
+  ⊢ |==> ∃ _ : gen_networkGS L V Σ, gen_network_interp σ.
+Proof.
+  iMod (own_alloc (gmap_view_auth 1 (σ : gmap L (leibnizO V)))) as (γ) "Hσ".
+  { exact: gmap_view_auth_valid.  }
+  iExists (GenNetworkGS _ _ _ γ).
+  done.
+Qed.
