primitive_laws.v
@@ -1,0 +1,20 @@
+From iris.program_logic Require Export ectx_lifting weakestpre.
+From iris.proofmode Require Import tactics.
+From chanlang Require Import lang notation network_ra.
+From iris Require Import options.
+
+(* Ghost state for reasoning about chan_lang threadpool. *)
+Class chanG Σ :=
+  ChanG {
+      chan_invG : invG Σ;
+      chan_gen_networkG :> gen_networkGS chan_id (option (gset val)) Σ;
+    }.
+
+Global Instance chan_irisG `{!chanG Σ} : irisG chan_lang Σ :=
+  {
+  iris_invG := chan_invG;
+  state_interp σ _ κs _ := (gen_network_interp σ.(chan))%I;
+  fork_post _ := True%I;
+  num_laters_per_step _ := 0;
+  state_interp_mono _ _ _ _ := fupd_intro _ _
+}.
